theories/examples/compression.v
@@ -1,0 +1,290 @@
+From iris.proofmode Require Import coq_tactics reduction spec_patterns.
+From iris.proofmode Require Export tactics.
+From iris.prelude Require Import options.
+From melocoton Require Import named_props.
+From melocoton.c_lang Require Import mlang_instantiation lang_instantiation.
+From melocoton.c_lang Require notation proofmode.
+
+Section SemBuffers.
+(* Of course, snappy is more complicated than this ..*)
+Definition buffer := list Z.
+
+Fixpoint compress_buffer (b:buffer) : buffer := (match b with
+| 0 :: 0 :: xs => 0 :: compress_buffer xs
+| x :: xs => 1 :: x :: compress_buffer xs
+| nil => nil end)%Z.
+
+Definition buffer_max_len (n : nat) := 2 * n.
+
+Fixpoint decompress_buffer (b:buffer) : option buffer := (match b with
+| 0 :: xs => option_map (λ x, 0 :: 0 :: x) (decompress_buffer xs)
+| 1 :: 0 :: 1 :: 0 :: xs => None
+| 1 :: 0 :: 0 :: xs => None
+| 1 :: x :: xs => option_map (cons x) (decompress_buffer xs)
+| nil => Some nil
+| _ => None end)%Z.
+
+Lemma decompress_compress b : decompress_buffer (compress_buffer b) = Some b.
+Proof.
+  induction b using (induction_ltof1 _ (@length _)); unfold ltof in *.
+  destruct x as [|b1 [|b2 br]].
+  - done.
+  - cbn. by case_match.
+  - cbn. repeat (case_match; try done).
+    all: cbn; rewrite H; last (cbn; lia); try done.
+Qed.
+
+Lemma decompress_to_nil b : decompress_buffer b = Some nil → b = nil.
+Proof.
+  destruct b; try done; cbn.
+  repeat (cbn in *; unfold option_map in *; case_match; simplify_eq; try done).
+Qed.
+
+Lemma compress_decompress b b2 : decompress_buffer b = Some b2 → compress_buffer b2 = b.
+Proof. revert b2.
+  induction b using (induction_ltof1 _ (@length _)); unfold ltof in *; intros bb Hb.
+  destruct x as [|b1 br].
+  - cbn in *. by simplify_eq.
+  - repeat (cbn in *; case_match; simplify_eq; try done); unfold option_map in *.
+    + case_match; last done.
+      simplify_eq. eapply H in H0; last (cbn; lia). subst br; done.
+    + case_match; last done. simplify_eq. eapply H in H0; last (cbn; lia).
+      destruct b; first done. cbn in *; repeat (case_match; simplify_eq); done.
+    + destruct (decompress_buffer l) eqn:Heq; cbn in *; last done. simplify_eq.
+      eapply H in Heq; last (cbn; lia). subst l. cbn. done.
+    + destruct (decompress_buffer l) eqn:Heq; cbn in *; last done. simplify_eq.
+      eapply H in Heq; last (cbn; lia). subst l. cbn. done.
+    + case_match; last done. simplify_eq.
+      eapply H in H0; last (cbn; lia). subst l. cbn. done.
+    + case_match; last done. simplify_eq.
+      eapply H in H0; last (cbn; lia). subst l. cbn. done.
+Qed.
+
+Lemma max_len_correct b : length (compress_buffer b) ≤ buffer_max_len (length b).
+Proof.
+  induction b using (induction_ltof1 _ (@length _)); unfold ltof in *.
+  destruct x as [|b1 [|b2 br]].
+  - cbn in *; lia.
+  - cbn. by case_match.
+  - cbn. repeat (case_match; try (first [done | cbn in *; lia])).
+    all: cbn in *; repeat (first [eapply le_n_S | erewrite Nat.add_succ_r]); etransitivity; first eapply H; cbn in *; lia.
+Qed.
+
+Lemma max_len_tight n : ∃ b, length b = n ∧ length (compress_buffer b) = buffer_max_len n.
+Proof.
+  induction n as [|n (b&IH1&IH2)].
+  - exists []. done.
+  - exists (1 :: b)%Z. cbn; split_and!; try done; try lia.
+    rewrite IH2. unfold buffer_max_len. lia.
+Qed.
+
+End SemBuffers.
+
+Section CBuffers.
+Import melocoton.c_lang.notation melocoton.c_lang.proofmode.
+
+Context `{SI:indexT}.
+Context `{!heapG_C Σ, !invG Σ}.
+
+Definition isBuffer (vl : list (option val)) (b : buffer) := vl = map (λ x:Z, Some (#x)) b.
+
+Definition buffy_max_len_name : string := "buffy_max_compressed_length".
+Definition buffy_max_len_code (inlen:expr) : expr := (BinOp MultOp inlen (#2))%CE.
+
+Definition buffy_compress_rec_name : string := "buffy_compress_rec".
+Definition buffy_compress_rec_code (inbuf inlen outbuf:expr) := (
+  if: inlen ≤ #0 then #0 else
+  if: inlen = #1
+    then ( outbuf <- #1 ;; outbuf +ₗ #1 <- *inbuf ;; #2 )
+    else if: ( *inbuf = #0) && ( *(inbuf +ₗ #1) = #0 )
+      then ( outbuf <- #0 ;; #1 + call: &buffy_compress_rec_name with (inbuf +ₗ #2, inlen - #2, outbuf +ₗ #1) )
+      else ( outbuf <- #1 ;; outbuf +ₗ #1 <- *inbuf ;; #2 + call: &buffy_compress_rec_name with (inbuf +ₗ #1, inlen - #1, outbuf +ₗ #2) ) )%CE.
+
+Definition buffy_compress_name : string := "buffy_compress".
+Definition buffy_compress_code (inbuf inlen outbuf outlenp:expr) := (
+  if: *outlenp < call: &buffy_max_len_name with (inlen) then #1 else
+    (outlenp <- call: &buffy_compress_rec_name with (inbuf, inlen, outbuf)) ;; #0 )%CE.
+
+Definition buffy_env : gmap string function := 
+  <[buffy_max_len_name      := Fun [BNamed "len"] (buffy_max_len_code "len")]> (
+  <[buffy_compress_rec_name := Fun [BNamed "inbuf"; BNamed "inlen"; BNamed "outbuf"] (buffy_compress_rec_code "inbuf" "inlen" "outbuf")]> (
+  <[buffy_compress_name     := Fun [BNamed "inbuf"; BNamed "inlen"; BNamed "outbuf"; BNamed "outlenp"]
+                                   (buffy_compress_code "inbuf" "inlen" "outbuf" "outlenp")]>
+  ∅)).
+
+Definition buffy_prog_env : prog_environ C_lang Σ := {|
+  penv_prog := buffy_env ;
+  penv_proto := λ _ _ _, False
+|}%I.
+
+Lemma buffy_max_len_spec E n (v:val) :
+  v = #(Z.of_nat n) →
+ (⊢ WP (call: &buffy_max_len_name with (Val v))%CE @ buffy_prog_env; E {{λ v', ⌜v' = #(Z.of_nat (buffer_max_len n))⌝}})%I.
+Proof.
+  iIntros (->). wp_pures. iModIntro. iPureIntro. do 2 f_equal. cbn. lia.
+Qed.
+
+Lemma ptr_offset_add (ℓ:loc) (z:Z) : bin_op_eval PtrOffsetOp #ℓ #z = Some (LitLoc (loc_add ℓ z)).
+Proof.
+  destruct ℓ; done.
+Qed.
+
+Lemma buffy_compress_rec_spec E ℓin ℓout vin bin vspace :
+   isBuffer vin bin →
+   length vspace ≥ buffer_max_len (length bin) →
+(⊢  ℓin  ↦C∗ vin
+ -∗ ℓout ↦C∗ vspace -∗
+    WP (call: &buffy_compress_rec_name with (Val #ℓin, Val #(length bin), Val #ℓout))%CE @ buffy_prog_env; E
+    {{ v', ∃ bout vout vrest,
+             ⌜isBuffer vout bout⌝
+           ∗ ⌜bout = compress_buffer bin⌝
+           ∗ ⌜v' = #(length vout)⌝
+           ∗ (∃ voverwritten, ⌜vspace = voverwritten ++ vrest⌝)
+           ∗ ℓout ↦C∗ (vout ++ vrest)
+           ∗ ℓin  ↦C∗ vin }})%I.
+Proof.
+  iIntros (HBuffer Hlength) "Hℓin Hℓout".
+  iLöb as "IH" forall (ℓin ℓout vin bin vspace HBuffer Hlength).
+  wp_pures.
+  destruct bin as [|bfst bin].
+  { cbn. rewrite bool_decide_decide. destruct decide; last lia.
+    wp_pures. iModIntro.
+    iExists [], [], vspace. iFrame. iPureIntro. split_and!; try done.
+    exists nil. done. }
+  cbn. rewrite bool_decide_decide. destruct decide; first lia.
+  wp_pures.
+  destruct bin as [|bsnd bin]; cbn; rewrite bool_decide_decide; destruct decide; try lia.
+  { iClear "IH". wp_pures. unfold isBuffer in *. subst vin. cbn.
+    iDestruct "Hℓin" as "(Hℓin&_)". cbn in Hlength.
+    destruct vspace as [|vs1 [|vs2 vsrest]]; cbn in Hlength; try lia.
+    cbn. iDestruct "Hℓout" as "(Hℓout1&Hℓout2&Hℓoutr)".
+    rewrite !loc_add_0.
+    wp_apply (wp_store with "Hℓout1"); iIntros "Hℓout1"; wp_pures.
+    wp_pure _. 1: apply ptr_offset_add.
+    wp_apply (wp_load with "Hℓin"); iIntros "Hℓin".
+    wp_apply (wp_store with "Hℓout2"); iIntros "Hℓout2"; wp_pures.
+    iModIntro. iExists [1%Z; bfst], _, vsrest.
+    iSplit; first done. cbn. rewrite !loc_add_0. iFrame. iPureIntro.
+    split_and!; try done.
+    1: by repeat case_match.
+    eexists [_; _]. done. }
+  wp_pures. unfold isBuffer in HBuffer. subst vin.
+  cbn in Hlength. rewrite !Nat.add_succ_r in Hlength. cbn.
+  iDestruct "Hℓin" as "(Hℓin0&Hℓin1&HℓinR)". rewrite !loc_add_0.
+  destruct (decide (bfst = 0 ∧ bsnd = 0)%Z) as [[-> ->]|Hnn].
+  { wp_apply (wp_load with "Hℓin0"); iIntros "Hℓin0"; wp_pures.
+    wp_pure _; first eapply ptr_offset_add.
+    wp_apply (wp_load with "Hℓin1"); iIntros "Hℓin1"; wp_pures.
+    destruct vspace as [|vsp1 vspr]; first (cbn in *; lia).
+    cbn. iDestruct "Hℓout" as "(Hℓou0&HℓouR)". rewrite !loc_add_0.
+    wp_apply (wp_store with "Hℓou0"); iIntros "Hℓou0"; wp_pures.
+    wp_pure _; first apply ptr_offset_add.
+    wp_pures. replace (Z.of_nat (S (S (length bin))) - 2)%Z with (Z.of_nat (length bin)) by lia.
+    wp_pure _; first apply ptr_offset_add.
+    wp_bind (FunCall _ _); wp_apply (wp_wand with "[HℓinR HℓouR]").
+    { iApply ("IH" with "[] [] [HℓinR]"); iClear "IH". 1: done.
+      2: { unfold array. iApply (big_sepL_wand with "HℓinR").
+           iApply big_sepL_intro. iIntros "!> % % % H". rewrite loc_add_assoc.
+           replace (Z.of_nat (S (S k))) with (2 + k)%Z by lia. done. }
+      2: { unfold array. iApply (big_sepL_wand with "HℓouR").
+           iApply big_sepL_intro. iIntros "!> % % % H". rewrite loc_add_assoc.
+           replace (Z.of_nat (S k)) with (1 + k)%Z by lia. done. }
+      iPureIntro. cbn in *. lia. }
+    { cbn. iClear "IH". unfold isBuffer.
+      iIntros (v) "(%bout&%vout&%vrest&->&->&->&(%vov&->)&HℓouR&HℓinR)".
+      wp_pures. iModIntro.
+      iExists (0%Z :: compress_buffer bin), _, vrest. iSplit; first done. iFrame.
+      repeat iSplit; try iPureIntro.
+      - done.
+      - cbn. do 2 f_equal. lia.
+      - cbn. by exists (vsp1 :: vov).
+      - unfold array. iApply (big_sepL_wand with "HℓinR").
+        iApply big_sepL_intro. iIntros "!> % % % H". rewrite loc_add_assoc.
+           replace (Z.of_nat (S (S k))) with (2 + k)%Z by lia. done.
+    }
+  }
+  { wp_bind (if: _ then _ else #0)%CE.
+    iApply (wp_wand _ _ _ (λ v, ⌜v = #0⌝ ∗ ℓin ↦C #bfst ∗ (ℓin +ₗ 1) ↦C #bsnd)%I with "[Hℓin0 Hℓin1]").
+    { wp_apply (wp_load with "Hℓin0"); iIntros "Hℓin0"; wp_pures.
+      rewrite bool_decide_decide. destruct decide.
+      { wp_pures; wp_pure _; first eapply ptr_offset_add.
+        wp_apply (wp_load with "Hℓin1"); iIntros "Hℓin1"; wp_pures.
+        rewrite bool_decide_decide. destruct decide; try lia.
+        iModIntro. iFrame. done. }
+      { wp_pures. iModIntro. iFrame. done. }
+    }
+    iIntros (?) "(->&Hℓin0&Hℓin1)". wp_pures.
+    destruct vspace as [|vsp1 [|vsp2 vspr]]; try (cbn in *; lia).
+    cbn. iDestruct "Hℓout" as "(Hℓou0&Hℓou1&HℓouR)". rewrite !loc_add_0.
+    wp_apply (wp_store with "Hℓou0"); iIntros "Hℓou0"; wp_pures.
+    wp_pure _; first eapply ptr_offset_add.
+    wp_apply (wp_load with "Hℓin0"); iIntros "Hℓin0"; wp_pures.
+    wp_apply (wp_store with "Hℓou1"); iIntros "Hℓou1"; wp_pures.
+    wp_pure _; first apply ptr_offset_add.
+    wp_pures. replace (Z.of_nat (S (S (length bin))) - 1)%Z with (Z.of_nat (S (length bin))) by lia.
+    wp_pure _; first apply ptr_offset_add.
+    wp_bind (FunCall _ _); iApply (wp_wand with "[Hℓin1 HℓinR HℓouR]").
+    { change (S (length bin)) with (length (bsnd :: bin)).
+      iApply ("IH" with "[] [] [Hℓin1 HℓinR]"); iClear "IH". 1: done.
+      2: { unfold array. cbn. rewrite !loc_add_assoc. iFrame.
+           iApply (big_sepL_wand with "HℓinR").
+           iApply big_sepL_intro. iIntros "!> % % % H". rewrite loc_add_assoc.
+           replace (Z.of_nat (S (S k))) with (1 + (S k))%Z by lia. done. }
+      2: { unfold array. iApply (big_sepL_wand with "HℓouR").
+           iApply big_sepL_intro. iIntros "!> % % % H". rewrite loc_add_assoc.
+           replace (Z.of_nat (S (S k))) with (2 + k)%Z by lia. done. }
+      iPureIntro. cbn in *. lia. }
+    { cbn. iClear "IH". unfold isBuffer.
+      iIntros (v) "(%bout&%vout&%vrest&->&->&->&(%vov&->)&HℓouR&Hℓin1&HℓinR)".
+      wp_pures. iModIntro.
+      iExists (1%Z :: bfst :: compress_buffer (bsnd :: bin)), _, vrest. iSplit; first done.
+      repeat iSplit; try iPureIntro. 4: cbn; iFrame.
+      - do 4 (cbn in *; case_match; try (exfalso; by eapply Hnn); simplify_eq; try congruence).
+      - cbn. do 2 f_equal. repeat case_match; cbn in *; lia.
+      - cbn. by exists (vsp1 :: vsp2 :: vov).
+      - rewrite !loc_add_0. iFrame "Hℓou0 Hℓin1". iSplitL "HℓouR".
+        + unfold array. iApply (big_sepL_wand with "HℓouR").
+          iApply big_sepL_intro. iIntros "!> % % % H". rewrite loc_add_assoc.
+          replace (Z.of_nat (S (S k))) with (2 + k)%Z by lia. done. 
+        + unfold array. iApply (big_sepL_wand with "HℓinR").
+          iApply big_sepL_intro. iIntros "!> % % % H". rewrite loc_add_assoc.
+           replace (Z.of_nat (S (S k))) with (1 + (S k))%Z by lia. done.
+    }
+  }
+Qed.
+
+Lemma buffy_compress_spec E ℓin ℓout ℓlen vin bin vspace :
+   isBuffer vin bin →
+   length vspace ≥ buffer_max_len (length bin) →
+(⊢  ℓin  ↦C∗ vin
+ -∗ ℓout ↦C∗ vspace
+ -∗ ℓlen ↦C  #(length vspace)
+ -∗ WP (call: &buffy_compress_name with (Val #ℓin, Val #(length bin), Val #ℓout, Val #ℓlen))%CE @ buffy_prog_env; E
+    {{ v', ∃ bout vout vrest,
+             ⌜isBuffer vout bout⌝
+           ∗ ⌜bout = compress_buffer bin⌝
+           ∗ ⌜v' = #0⌝
+           ∗ (∃ voverwritten, ⌜vspace = voverwritten ++ vrest⌝)
+           ∗ ℓout ↦C∗ (vout ++ vrest)
+           ∗ ℓin  ↦C∗ vin 
+           ∗ ℓlen ↦C  #(length vout)}})%I.
+Proof.
+  iIntros (HBuffer Hlength) "Hℓin Hℓout Hℓlen".
+  wp_pures.
+  wp_apply (wp_load with "Hℓlen"); iIntros "Hℓlen".
+  wp_bind (FunCall _ _).
+  iApply wp_wand. 1: iApply buffy_max_len_spec; first done. cbn.
+  iIntros (?) "->".
+  wp_pures. rewrite bool_decide_decide. destruct decide; cbn in *; try lia.
+  wp_pure _. wp_bind (FunCall _ _).
+  iApply (wp_wand with "[Hℓin Hℓout]").
+  1: by iApply (buffy_compress_rec_spec with "[Hℓin]").
+  cbn.
+  iIntros (v) "(%bout&%vout&%vrest&Hbuf&HH1&->&HH3&HℓouR&HℓinR)".
+  wp_apply (wp_store with "Hℓlen"); iIntros "Hℓlen".
+  wp_pures. iModIntro.
+  iExists bout, vout, vrest. by iFrame.
+Qed.
+
+End CBuffers.
+
